\section{Calculation for the limit for \texorpdfstring{$\wpfour$}{wprime4bar} as \texorpdfstring{$\delta$}{delta} goes to 1}
\label{sec:calculation-for-the-limit-for-wprime4bar-as-delta-goes-to-1}

\begin{align}
    \label{eq:limit_wprime4_delta_to_1_calc}
    \lim_{\substack{\delta \to 1, \\ \wpthree \to 0}}\left(\wpfour\right)
    &= \lim_{\substack{\delta \to 1, \\ \wpthree \to 0}}
    \left(\left(\wptwo\right)^2\right.
    \cancelto{0}{\frac{(1-\delta \lambda_w)^2}{(1-\delta)}}
    \left(3 \tsw^4 + 6 \tswfact \tsw^2 + \tswfact^2\right) \nonumber\\
    &\quad+ \frac{1}{\tswfact} \frac{1}{(1-\delta \lambda_w)}
    \frac{\left(\wpthree\right)^2}{\wptwo}
    + \left. \delta 3 \lambda_w^2 \left(\wptwo\right)^2\right)
    \\
    &= \lim_{\substack{\delta \to 1, \\ \wpthree \to 0}}
    \left(
    \frac{
        \left(\wpthree\right)^2
    }
    {
        \wptwo
        \left(\left(\frac{\wptwo (1-\delta\lambda_w) - \sigma_w^2 (1-\delta)}{\wptwo (1-\delta\lambda_w)}\right)\right)
        (1-\delta \lambda_w)
    }
    + 3 \delta \lambda_w^2 \left(\wptwo\right)^2
    \right)
    \\
    &= \lim_{\substack{\delta \to 1, \\ \wpthree \to 0}}
    \left(
    \frac{
        \left(\wpthree\right)^2
    }{
        \wptwo (1-\delta\lambda_w) - \sigma_w^2 (1-\delta)
    }
    + 3 \delta \lambda_w^2 \left(\wptwo\right)^2
    \right)
    \\
    &= \lim_{\substack{\delta \to 1, \\ \wpthree \to 0}}
    \left(
    \frac{
        \left(\wpthree\right)^2
    }{
        (1-\delta\lambda_w)
        \left(\wptwo - \sigma_w^2 \underbrace{\left(\frac{1-\delta}{1-\delta\lambda_w}\right)}_{\to \frac{1}{2 - c_1}}\right)
    }
    + 3 \delta \lambda_w^2 \left(\wptwo\right)^2
    \right)
    \\
    &= \lim_{\substack{\delta \to 1, \\ \wpthree \to 0}}
    \left(
    \frac{
        \left(\wpthree\right)^2
    }{
        (1 - \delta\lambda_w)
        \left(\wptwo - \frac{\sigma_w^2}{2 - c_1}\right)
    }
    \right.
    \nonumber\\
    &\quad+
    \left.3 \delta \left(c_1^2\delta^2 - 2c_1^2\delta + c_1^2 - 2c_1\delta^2 + 2c_1\delta + \delta^2\right) \left(\wptwo\right)^2
    \right)
    \\
    &= \lim_{\substack{\delta \to 1, \\ \wpthree \to 0}}
    \left(
    \frac{
        \left(\wpthree\right)^2
    }{
        (1 - \delta\lambda_w)
        \left(\wptwo - \frac{\sigma_w^2}{2 - c_1}\right)
    }
    \right)
    + 3 \left(\wptwo\right)^2
\end{align}
Now, we use \cref{eq:delta_propto}, saying that $1-\delta$ \enquote{goes as} skeweness.
This also implies that $1-\delta\lambda_w$ \enquote{goes as} skeweness.
\begin{align}
    \lim_{\substack{\delta \to 1, \\ \wpthree \to 0}}
    \left(\wpfour\right)
    &= \lim_{\substack{\delta \to 1, \\ \wpthree \to 0}}
    \left(
    \frac{
        \left(\wpthree\right)^2
    }{
        \left(\frac{\wpthree}{\wptwo^{3/2}}\right)
        \left(\wptwo - \frac{\sigma_w^2}{2 - c_1}\right)
    }
    \right)
    + 3 \left(\wptwo\right)^2
    \\
    &=
    \left(
    \frac{
        \left(\wpthree\right)^2
        \wptwo^{3/2}
    }{
        \wpthree
        \left(\wptwo - \frac{\sigma_w^2}{2 - c_1}\right)
    }
    \right)
    + 3 \left(\wptwo\right)^2
    \\
    &=
    \cancelto{0}{
        \left(
        \frac{
            \wpthree
            \;
            \wptwo^{3/2}
        }{
            \left(\wptwo - \frac{\sigma_w^2}{2 - c_1}\right)
        }
        \right)
    }
    + 3 \left(\wptwo\right)^2
    \\
    &= 3 \left(\wptwo\right)^2.
\end{align}


