\section{Calculation for the limit for \texorpdfstring{$\wptwothlp$}{wprime2thetalprimebar} as \texorpdfstring{$\delta$}{delta} goes to 1}
\label{sec:calculation-for-the-limit-for-wprime2thetalprimebar-as-delta-goes-to-1}

\begin{align}
    \label{eq:limit_wprime2thetalbar_delta_to_1_calc}
    \lim_{\delta \to 1}\left(\wptwothlp\right)
    &= \lim_{\delta \to 1}\left(
    \frac{1}{\tswfact}
    \quad
    \frac{1 - \delta \lambda_{w\theta}}{1-\delta \lambda_w}
    \frac{\overline{w'^3}}{\overline{w'^2}} \overline{w'\theta_l'}
    \right)
    \\
    &= \lim_{\delta \to 1}\left(
    \frac{(1 - \delta \lambda_{w\theta}) \cdot \overline{w'^3} \cdot \overline{w'\theta_l'}}
    {(1-\delta \lambda_w)\overline{w'^2} (1-\frac{\sigma_w^2 (1-\delta)}{\wptwo (1-\delta\lambda_w)})}
    \right)
    \\
    &= \lim_{\delta \to 1}\left(
    \underbrace{\left(\frac{1 - \delta \lambda_{w\theta}}{1 - \delta\lambda_w}\right)}_{\to \frac{-2 + c_1}{-2 + c_2}}
    \frac{\overline{w'^3} \cdot \overline{w'\theta_l'}}
    {\left(\wptwo - \sigma_w^2 \underbrace{\left(\frac{1-\delta}{1-\delta\lambda_w}\right)}_{\to \frac{1}{2 - c_1}}\right)}
    \right)
    \\
    &= \frac{-2 + c_1}{-2 + c_2} \cdot
    \frac{\overline{w'^3} \cdot \overline{w'\theta_l'}}
    {\wptwo - \frac{\sigma_w^2}{2 - c_1}}
    = \frac{\overline{w'^3} \cdot \overline{w'\theta_l'} \cdot (c_1 - 2)}
    {(c_2 - 2)\wptwo - \frac{(c_2 - 2)\sigma_w^2}{2 - c_1}} \\
    &= \frac{\overline{w'^3} \cdot \overline{w'\theta_l'} \cdot (c_1 - 2)}
    {\frac{(2 - c_1) (\wptwo c_2 - 2\wptwo) - \sigma_w^2 c_2 + 2\sigma_w^2}{2 - c_1}}
    = \frac{\overline{w'^3} \cdot \overline{w'\theta_l'} \cdot (c_1 - 2)}
    {\frac{2\wptwo c_2 - 4\wptwo - c_1 c_2 \wptwo + 2 c_1 \wptwo - \sigma_w^2 c_2 + 2\sigma_w^2}{2 - c_1}} \\
    &= \frac{\overline{w'^3} \cdot \overline{w'\theta_l'} \cdot (c_1 - 2) \cdot (2 - c_1)}
    {2\wptwo c_2 - 4\wptwo - c_1 c_2 \wptwo + 2 c_1 \wptwo - \sigma_w^2 c_2 + 2\sigma_w^2} \\
    &= \frac{\overline{w'^3} \cdot \overline{w'\theta_l'} \cdot (c_1 - 2) \cdot (2 - c_1)}
    {(2 - c_2) (c_1\wptwo + \sigma_w^2 - 2\wptwo)}
\end{align}